feat: Implement formal Coq proofs for Parser Error Recovery and strict termination

bin/lexer.ml
@@ -1,15 +1,5 @@
 open Compiler_lib.Compiler
 
-type token =
-  | TId of string
-  | TInt of string
-  | TStr of string
-  | TSym of string
-  | TEOF
-  | TComment of string
-
-type token_with_span = token * span
-
 let is_alpha c =
   (c >= 'a' && c <= 'z') || (c >= 'A' && c <= 'Z') || c = '_'
 
@@ -31,19 +21,18 @@ let make_span file_name start_idx _end_idx =
 let tokenize filename source =
   let len = String.length source in
   let rec aux i acc =
-    if i >= len then List.rev ((TEOF, make_span filename i i) :: acc)
+    if i >= len then List.rev (TokEOF (make_span filename i i) :: acc)
     else
       let c = source.[i] in
       if c = ' ' || c = '\n' || c = '\r' || c = '\t' then aux (i + 1) acc
       else if c = '/' && i + 1 < len && source.[i + 1] = '/' then
-        (* Comment *)
         let start_idx = i in
         let rec consume_comment j =
           if j >= len || source.[j] = '\n' then j else consume_comment (j + 1)
         in
         let _end_idx = consume_comment i in
         let text = String.sub source start_idx (_end_idx - start_idx) in
-        aux _end_idx ((TComment text, make_span filename start_idx _end_idx) :: acc)
+        aux _end_idx (TokComment (char_list_of_string text, make_span filename start_idx _end_idx) :: acc)
       else if is_alpha c then
         let start_idx = i in
         let rec consume_id j =
@@ -51,7 +40,7 @@ let tokenize filename source =
         in
         let _end_idx = consume_id i in
         let text = String.sub source start_idx (_end_idx - start_idx) in
-        aux _end_idx ((TId text, make_span filename start_idx _end_idx) :: acc)
+        aux _end_idx (TokId (char_list_of_string text, make_span filename start_idx _end_idx) :: acc)
       else if is_digit c then
         let start_idx = i in
         let rec consume_int j =
@@ -59,7 +48,7 @@ let tokenize filename source =
         in
         let _end_idx = consume_int i in
         let text = String.sub source start_idx (_end_idx - start_idx) in
-        aux _end_idx ((TInt text, make_span filename start_idx _end_idx) :: acc)
+        aux _end_idx (TokInt (char_list_of_string text, make_span filename start_idx _end_idx) :: acc)
       else if c = '"' then
         let start_idx = i in
         let rec consume_str j =
@@ -69,14 +58,14 @@ let tokenize filename source =
         in
         let _end_idx = consume_str (i + 1) in
         let text = String.sub source (start_idx + 1) (_end_idx - start_idx - 2) in
-        aux _end_idx ((TStr text, make_span filename start_idx _end_idx) :: acc)
+        aux _end_idx (TokStr (char_list_of_string text, make_span filename start_idx _end_idx) :: acc)
       else if c = '=' && i + 1 < len && source.[i + 1] = '=' then
-        aux (i + 2) ((TSym "==", make_span filename i (i + 2)) :: acc)
+        aux (i + 2) (TokSym (char_list_of_string "==", make_span filename i (i + 2)) :: acc)
       else if c = '=' && i + 1 < len && source.[i + 1] = '>' then
-        aux (i + 2) ((TSym "=>", make_span filename i (i + 2)) :: acc)
+        aux (i + 2) (TokSym (char_list_of_string "=>", make_span filename i (i + 2)) :: acc)
       else if c = '-' && i + 1 < len && source.[i + 1] = '>' then
-        aux (i + 2) ((TSym "->", make_span filename i (i + 2)) :: acc)
+        aux (i + 2) (TokSym (char_list_of_string "->", make_span filename i (i + 2)) :: acc)
       else
-        aux (i + 1) ((TSym (String.make 1 c), make_span filename i (i + 1)) :: acc)
+        aux (i + 1) (TokSym (char_list_of_string (String.make 1 c), make_span filename i (i + 1)) :: acc)
   in
   aux 0 []
