bin/main.ml
@@ -76,5 +76,5 @@ let () =
   print_endline "\n[Error Recovery Parser Test]";
   let source = "x; y; @@; z; 42" in
   let tokens = Lexer.tokenize "test_error.chester" source in
-  let cst = Parser.parse tokens in
+  let cst = parse tokens in
   print_endline (string_of_char_list (format_cst 100 0 cst))
